Start to unify ground and non-ground ordering

Superposition_Calculus/Ground_Ordering.thy
@@ -4,22 +4,20 @@ theory Ground_Ordering
     Transitive_Closure_Extra
     Clausal_Calculus_Extra
     Min_Max_Least_Greatest_Multiset
+    Clause_Ordering
 begin
 
-locale ground_ordering =
-  fixes
-    less_trm :: "'f gterm \<Rightarrow> 'f gterm \<Rightarrow> bool" (infix "\<prec>\<^sub>t" 50)
+locale ground_ordering = clause_ordering less_trm
+  for
+    less_trm :: "'f gterm \<Rightarrow> 'f gterm \<Rightarrow> bool" (infix "\<prec>\<^sub>t" 50) +
   assumes
-    transp_less_trm[intro]: "transp (\<prec>\<^sub>t)" and
-    asymp_less_trm[intro]: "asymp (\<prec>\<^sub>t)" and
+    (* transp_less_trm[intro]: "transp (\<prec>\<^sub>t)" and *)
+    (* asymp_less_trm[intro]: "asymp (\<prec>\<^sub>t)" and *)
     wfP_less_trm[intro]: "wfP (\<prec>\<^sub>t)" and
     totalp_less_trm[intro]: "totalp (\<prec>\<^sub>t)" and
     less_trm_compatible_with_gctxt[simp]: "\<And>ctxt t t'. t \<prec>\<^sub>t t' \<Longrightarrow> ctxt\<langle>t\<rangle>\<^sub>G \<prec>\<^sub>t ctxt\<langle>t'\<rangle>\<^sub>G" and
     less_trm_if_subterm[simp]: "\<And>t ctxt. ctxt \<noteq> \<box>\<^sub>G \<Longrightarrow> t \<prec>\<^sub>t ctxt\<langle>t\<rangle>\<^sub>G"
 begin
-
-lemma irreflp_on_less_trm[simp]: "irreflp_on A (\<prec>\<^sub>t)"
-  by (metis asympD asymp_less_trm irreflp_onI)
 
 abbreviation lesseq_trm (infix "\<preceq>\<^sub>t" 50) where
   "lesseq_trm \<equiv> (\<prec>\<^sub>t)\<^sup>=\<^sup>="
@@ -28,43 +26,18 @@ lemma lesseq_trm_if_subtermeq: "t \<preceq>\<^sub>t ctxt\<langle>t\<rangle>\<^su
   using less_trm_if_subterm
   by (metis gctxt_ident_iff_eq_GHole reflclp_iff)
 
-definition less_lit :: "'f gatom literal \<Rightarrow> 'f gatom literal \<Rightarrow> bool" (infix "\<prec>\<^sub>l" 50) where
-  "less_lit L1 L2 \<equiv> multp (\<prec>\<^sub>t) (mset_lit L1) (mset_lit L2)"
-
 abbreviation lesseq_lit (infix "\<preceq>\<^sub>l" 50) where
   "lesseq_lit \<equiv> (\<prec>\<^sub>l)\<^sup>=\<^sup>="
 
-abbreviation less_cls :: "'f gatom clause \<Rightarrow> 'f gatom clause \<Rightarrow> bool" (infix "\<prec>\<^sub>c" 50) where
-  "less_cls \<equiv> multp (\<prec>\<^sub>l)"
-
 abbreviation lesseq_cls (infix "\<preceq>\<^sub>c" 50) where
   "lesseq_cls \<equiv> (\<prec>\<^sub>c)\<^sup>=\<^sup>="
-
-lemma transp_on_less_lit[simp]: "transp_on A (\<prec>\<^sub>l)"
-  by (smt (verit, ccfv_SIG) less_lit_def transpE transp_less_trm transp_multp transp_onI)
-
-corollary transp_less_lit: "transp (\<prec>\<^sub>l)"
-  by simp
-
-lemma transp_less_cls[simp]: "transp (\<prec>\<^sub>c)"
-  by (simp add: transp_multp)
-
-lemma asymp_on_less_lit[simp]: "asymp_on A (\<prec>\<^sub>l)"
-  by (metis asympD asymp_less_trm asymp_multp\<^sub>H\<^sub>O asymp_onI less_lit_def multp_eq_multp\<^sub>H\<^sub>O
-      transp_less_trm)
-
-corollary asymp_less_lit: "asymp (\<prec>\<^sub>l)"
-  by simp
-
-lemma asymp_less_cls[simp]: "asymp (\<prec>\<^sub>c)"
-  by (simp add: asymp_multp\<^sub>H\<^sub>O multp_eq_multp\<^sub>H\<^sub>O)
 
 lemma wfP_less_lit[simp]: "wfP (\<prec>\<^sub>l)"
   unfolding less_lit_def
   using wfP_less_trm wfP_multp wfP_if_convertible_to_wfP by meson
 
 lemma wfP_less_cls[simp]: "wfP (\<prec>\<^sub>c)"
-  using wfP_less_lit wfP_multp by blast
+  using wfP_less_lit wfP_multp less_cls_def by metis
 
 lemma totalp_on_less_lit[simp]: "totalp_on A (\<prec>\<^sub>l)"
 proof (rule totalp_onI)
@@ -89,10 +62,8 @@ proof (rule totalp_onI)
   qed
 qed
 
-corollary totalp_less_lit: "totalp (\<prec>\<^sub>l)"
-  by simp
-
 lemma totalp_less_cls[simp]: "totalp (\<prec>\<^sub>c)"
+  unfolding less_cls_def
 proof (rule totalp_multp)
   show "totalp (\<prec>\<^sub>l)"
     by simp
@@ -101,56 +72,20 @@ next
     by simp
 qed
 
-sublocale linorder_trm: linorder lesseq_trm less_trm
+sublocale term_order: linorder lesseq_trm less_trm
 proof unfold_locales
-  show "\<And>x y. (x \<prec>\<^sub>t y) = (x \<preceq>\<^sub>t y \<and> \<not> y \<preceq>\<^sub>t x)"
-    by (metis asympD asymp_less_trm reflclp_iff)
-next
-  show "\<And>x. x \<preceq>\<^sub>t x"
-    by simp
-next
-  show "\<And>x y z. x \<preceq>\<^sub>t y \<Longrightarrow> y \<preceq>\<^sub>t z \<Longrightarrow> x \<preceq>\<^sub>t z"
-    by (meson transpE transp_less_trm transp_on_reflclp)
-next
-  show "\<And>x y. x \<preceq>\<^sub>t y \<Longrightarrow> y \<preceq>\<^sub>t x \<Longrightarrow> x = y"
-    by (metis asympD asymp_less_trm reflclp_iff)
-next
   show "\<And>x y. x \<preceq>\<^sub>t y \<or> y \<preceq>\<^sub>t x"
     by (metis reflclp_iff totalpD totalp_less_trm)
 qed
 
-sublocale linorder_lit: linorder lesseq_lit less_lit
+sublocale literal_order: linorder lesseq_lit less_lit
 proof unfold_locales
-  show "\<And>x y. (x \<prec>\<^sub>l y) = (x \<preceq>\<^sub>l y \<and> \<not> y \<preceq>\<^sub>l x)"
-    by (metis asympD asymp_less_lit reflclp_iff)
-next
-  show "\<And>x. x \<preceq>\<^sub>l x"
-    by simp
-next
-  show "\<And>x y z. x \<preceq>\<^sub>l y \<Longrightarrow> y \<preceq>\<^sub>l z \<Longrightarrow> x \<preceq>\<^sub>l z"
-    by (meson transpE transp_less_lit transp_on_reflclp)
-next
-  show "\<And>x y. x \<preceq>\<^sub>l y \<Longrightarrow> y \<preceq>\<^sub>l x \<Longrightarrow> x = y"
-    by (metis asympD asymp_less_lit reflclp_iff)
-next
   show "\<And>x y. x \<preceq>\<^sub>l y \<or> y \<preceq>\<^sub>l x"
-    by (metis reflclp_iff totalpD totalp_less_lit)
+    by (metis reflclp_iff totalpD totalp_on_less_lit)
 qed
 
-sublocale linorder_cls: linorder lesseq_cls less_cls
+sublocale clause_order: linorder lesseq_cls less_cls
 proof unfold_locales
-  show "\<And>x y. (x \<prec>\<^sub>c y) = (x \<preceq>\<^sub>c y \<and> \<not> y \<preceq>\<^sub>c x)"
-    by (metis asympD asymp_less_cls reflclp_iff)
-next
-  show "\<And>x. x \<preceq>\<^sub>c x"
-    by simp
-next
-  show "\<And>x y z. x \<preceq>\<^sub>c y \<Longrightarrow> y \<preceq>\<^sub>c z \<Longrightarrow> x \<preceq>\<^sub>c z"
-    by (meson transpE transp_less_cls transp_on_reflclp)
-next
-  show "\<And>x y. x \<preceq>\<^sub>c y \<Longrightarrow> y \<preceq>\<^sub>c x \<Longrightarrow> x = y"
-    by (metis asympD asymp_less_cls reflclp_iff)
-next
   show "\<And>x y. x \<preceq>\<^sub>c y \<or> y \<preceq>\<^sub>c x"
     by (metis reflclp_iff totalpD totalp_less_cls)
 qed
@@ -201,15 +136,15 @@ lemma context_less_term_lesseq:
     "\<And>t. ctxt\<langle>t\<rangle>\<^sub>G \<prec>\<^sub>t ctxt'\<langle>t\<rangle>\<^sub>G"
     "t \<preceq>\<^sub>t t'"
   shows "ctxt\<langle>t\<rangle>\<^sub>G \<prec>\<^sub>t ctxt'\<langle>t'\<rangle>\<^sub>G"
-  using assms less_trm_compatible_with_gctxt linorder_trm.dual_order.strict_trans 
-  by blast
+  using assms less_trm_compatible_with_gctxt
+  by (metis reflclp_iff term_order.dual_order.strict_trans)
 
 lemma context_lesseq_term_less:
   assumes 
     "\<And>t. ctxt\<langle>t\<rangle>\<^sub>G \<preceq>\<^sub>t ctxt'\<langle>t\<rangle>\<^sub>G"
     "t \<prec>\<^sub>t t'"
   shows "ctxt\<langle>t\<rangle>\<^sub>G \<prec>\<^sub>t ctxt'\<langle>t'\<rangle>\<^sub>G"
-  using assms less_trm_compatible_with_gctxt linorder_trm.dual_order.strict_trans1 
+  using assms less_trm_compatible_with_gctxt term_order.dual_order.strict_trans1 
   by blast
 
 end
